Defines a function to get a bag from a bootstrap binomial heap
In order to prove the functional correctness of bootstraped
binomial heaps, we need a function to transform them into
bags.

To prove the termination of this function, I introduced another
function that computes the size of a bootstraped binomial heap.
This function counts the number of bootstraped heaps (empty or
not) that occur inside a bootstraped heap.

I had to verify some properties on this size function to prove
the termination.

translator/okasaki-examples/SkewBinomialHeapScript.sml
@@ -195,6 +195,28 @@ val b_delete_min_def = Define `
     SOME (Bsbheap smallest_root (merge (b_heap_comparison geq) rest smallest_children)))
 `;
 
+val b_heap_size_def = Define `
+  (b_heap_size f Bsbempty = (1:num)) /\
+  (b_heap_size f (Bsbheap e c) = 1 + (f e + b_heap1_size f c)) /\
+  (b_heap1_size f [] = 0) /\
+  (b_heap1_size f (t::ts) = (b_heap2_size f t) + (b_heap1_size f ts)) /\
+  (b_heap2_size f (Sbnode x r a c) =
+     (b_heap_size f x) + (b_heap3_size f a) + (b_heap4_size f c)) /\
+  (b_heap3_size f [] = 0) /\
+  (b_heap3_size f (e::es) = (b_heap_size f e) + (b_heap3_size f es)) /\
+  (b_heap4_size f [] = 0) /\
+  (b_heap4_size f (t::ts) = (b_heap2_size f t) + (b_heap4_size f ts))
+`;
+
+val b_heap_to_bag_defn = Hol_defn "b_heap_to_bag" `
+  (b_heap_to_bag _ Bsbempty = {||}) /\
+  (b_heap_to_bag geq (Bsbheap r c) =
+    if c = [] then {|r|} else
+    let min = THE (find_min (b_heap_comparison geq) c) in
+    let rest = THE (delete_min (b_heap_comparison geq) c) in
+    BAG_UNION (b_heap_to_bag geq min) (b_heap_to_bag geq (Bsbheap r rest)))
+`;
+
 (* Useful lemmas *)
 Theorem rank_irrelevance_bag:
   !root r1 r2 aux ch. tree_to_bag (Sbnode root r1 aux ch) = tree_to_bag (Sbnode root r2 aux ch)
@@ -555,17 +577,16 @@ find_min returns the smallest element with the highest
 priority of the heap.
 *)
 Theorem find_min_exists:
-  !geq h. WeakLinearOrder geq /\
-          h <> [] ==>
+  !geq h. h <> [] ==>
           (find_min geq h) <> NONE
 Proof
   Induct_on `h`
   >- rw[]
   >- (Cases_on `h` \\
      rw[find_min_def] \\
-     res_tac \\
-     Cases_on `find_min geq (h'::t)` \\
-     rw[])
+     Cases_on `find_min geq (h'::t)`
+     >- res_tac
+     >- rw[])
 QED;
 
 Theorem find_min_bag:
@@ -760,6 +781,204 @@ Proof
       rw[tree_to_bag_general] \\
       metis_tac[COMM_BAG_UNION, ASSOC_BAG_UNION, reverse_bag])
 QED;
+
+(* Proof that b_heap_to_bag is terminating *)
+Theorem root_size:
+  !f t. b_heap_size f (root t) <= b_heap2_size f t
+Proof
+  Cases_on `t` \\
+  rw[root_def, b_heap_size_def]
+QED;
+
+Theorem find_min_size:
+  !geq c f. c <> [] ==> b_heap_size f (THE (find_min geq c)) <= b_heap1_size f c
+Proof
+  rpt strip_tac \\
+  Induct_on `c`
+  >- rw[]
+  >- (rpt strip_tac \\
+      Cases_on `c`
+      >- (rw[find_min_def, b_heap_size_def] \\
+          `b_heap_size f (root h) <= b_heap2_size f h`
+          by rw[root_size] \\
+	  rw[])
+      >- (rw[find_min_def, b_heap_size_def] \\
+          Cases_on `find_min geq (h'::t)`
+          >- fs[find_min_exists]
+	  >- (rw[]
+              >- (`b_heap_size f (root h) <= b_heap2_size f h`
+                  by rw[root_size] \\
+                  rw[])
+	      >- fs[THE_DEF])))
+QED;
+
+Theorem equiv_size1_size4:
+  !h f. b_heap1_size f h = b_heap4_size f h
+Proof
+  Induct_on `h` \\
+  rw[b_heap_size_def]
+QED;
+
+Theorem app_size:
+  !f h1 h2. b_heap4_size f (h1 ++ h2) = b_heap4_size f h1 + b_heap4_size f h2
+Proof
+  Induct_on `h1`
+  >- rw[APPEND_NIL, b_heap_size_def]
+  >- rw[APPEND, b_heap_size_def]
+QED;
+
+Theorem rev_size:
+  !f h. b_heap4_size f (REVERSE h) = b_heap4_size f h
+Proof
+  Induct_on `h`
+  >- rw[REVERSE, b_heap_size_def]
+  >- rw[REVERSE_DEF, app_size, b_heap_size_def]
+QED;
+
+Theorem link_size:
+  !geq f h1 h2. b_heap2_size f (tree_link geq h1 h2) = b_heap2_size f h1 + b_heap2_size f h2
+Proof
+  Cases_on `h1` \\
+  Cases_on `h2` \\
+  rw[tree_link_def] \\
+  rw[b_heap_size_def]
+QED;
+
+Theorem skew_link_size:
+  !geq f e h1 h2.
+    b_heap2_size f (skew_link geq e h1 h2) =
+    b_heap_size f e + b_heap2_size f h1 + b_heap2_size f h2
+Proof
+  rw[skew_link_def, b_heap_size_def] \\
+  Cases_on `h1` \\
+  Cases_on `h2` \\
+  rw[root_def, rank_def, children_def, aux_def, tree_link_def, b_heap_size_def]
+QED;
+
+Theorem insert_size:
+  !f e h geq. b_heap1_size f (insert geq e h) = (b_heap_size f e) + (b_heap1_size f h)
+Proof
+  Cases_on `h`
+  >- rw[insert_def, leaf_def, b_heap_size_def]
+  >- (Cases_on `t`
+      >- rw[insert_def, leaf_def, b_heap_size_def]
+      >- (rw[insert_def, b_heap_size_def] \\
+          rw[skew_link_size, leaf_def, b_heap_size_def]))
+QED;
+
+Theorem insert_list_size:
+  !geq f l1 l2. b_heap1_size f (insert_list geq l1 l2) = (b_heap3_size f l1) + (b_heap1_size f l2)
+Proof
+  Induct_on `l1`
+  >- rw[insert_list_def, b_heap_size_def]
+  >- rw[insert_list_def, b_heap_size_def, insert_size]
+QED;
+
+Theorem bheap_size_not_zero:
+  !f h. 0 < b_heap_size f h
+Proof
+  Cases_on `h`
+  >- rw[b_heap_size_def]
+  >- rw[b_heap_size_def]
+QED;
+
+Theorem insert_aux_rev_children_size:
+  !geq h f. b_heap1_size f (insert_list geq (aux h) (REVERSE (children h)))
+             <  b_heap2_size f h
+Proof
+  Cases_on `h` \\
+  rw[aux_def, children_def] \\
+  Induct_on `l0`
+  >- (rw[insert_list_def, b_heap_size_def] \\
+      Cases_on `l`
+      >- rw[REVERSE, b_heap_size_def, bheap_size_not_zero]
+      >- rw[equiv_size1_size4, app_size, rev_size,
+	    b_heap_size_def, bheap_size_not_zero])
+  >- (rw[insert_size,insert_list_def, b_heap_size_def, insert_list_size,
+         rev_size, equiv_size1_size4, bheap_size_not_zero])
+QED;
+
+Theorem get_min_size:
+  !geq q r f h. h <> [] /\ get_min geq h = (q,r) ==>
+          b_heap1_size f h = b_heap2_size f q + b_heap1_size f r
+Proof
+  Induct_on `h`
+  >- rw[]
+  >- (Cases_on `h`
+      >- (rw[get_min_def, b_heap_size_def] \\ rw[b_heap_size_def])
+      >- (Cases_on `get_min geq (h'::t)` \\
+          `h'::t <> []` by rw[] \\
+	  res_tac \\
+          rw[get_min_def] \\
+          Cases_on `get_min geq' (h'::t)` \\
+          fs[] \\
+          Cases_on `geq' (root q'') (root h)`
+          >- (fs[] \\
+              rw[b_heap_size_def])
+	  >- (fs[] \\
+              res_tac \\
+              rw[b_heap_size_def])))
+QED;
+
+Theorem binomial_insert_size:
+  !geq f t h. b_heap1_size f (binomial_insert geq t h) = (b_heap2_size f t) + (b_heap1_size f h)
+Proof
+  Induct_on `h`
+  >- rw[binomial_insert_def, b_heap_size_def]
+  >- (rw[binomial_insert_def, b_heap_size_def] \\
+      rw[link_size])
+QED;
+
+Theorem normalize_size:
+  !geq f h. b_heap1_size f (normalize geq h) = b_heap1_size f h
+Proof
+  Cases_on `h`
+  >- rw[normalize_def, b_heap_size_def]
+  >- rw[normalize_def, b_heap_size_def, binomial_insert_size]
+QED;
+
+Theorem merge_tree_size:
+  !geq f h1 h2. b_heap1_size f (merge_tree geq h1 h2) = (b_heap1_size f h1) + (b_heap1_size f h2)
+Proof
+  Induct_on `h1` \\
+  Induct_on `h2`
+  >- rw[merge_tree_def, b_heap_size_def]
+  >- rw[merge_tree_def, b_heap_size_def]
+  >- rw[merge_tree_def, b_heap_size_def]
+  >- rw[merge_tree_def, b_heap_size_def,
+        binomial_insert_size, link_size]
+QED;
+
+Theorem delete_min_size:
+  !geq c f. c <> [] ==> b_heap1_size f (THE (delete_min geq c)) < b_heap1_size f c
+Proof
+  Cases_on `c` \\
+  rpt strip_tac
+  >- rw[]
+  >- (rpt strip_tac \\
+      Cases_on `t`
+      >- (rw[delete_min_def, get_min_def, b_heap_size_def,
+	     normalize_def, merge_tree_def, insert_aux_rev_children_size])
+      >- (rw[delete_min_def, b_heap_size_def] \\
+          Cases_on `get_min geq (h::h'::t')` \\
+          `h::h'::t' <> []` by rw[] \\
+          imp_res_tac get_min_size \\
+          fs[b_heap_size_def] \\
+          rw[insert_list_size, merge_tree_size, normalize_size] \\
+          rw[equiv_size1_size4, rev_size, normalize_size] \\
+	  Cases_on `q` \\
+          rw[aux_def, children_def, b_heap_size_def, bheap_size_not_zero]))
+QED;
+
+val (b_heap_to_bag_def, b_heap_to_bag_ind) =
+  Defn.tprove (b_heap_to_bag_defn,
+    WF_REL_TAC `measure (\ (_, h). b_heap_size (\x.0) h)` \\
+    rpt strip_tac
+    >- (imp_res_tac find_min_size \\
+        rw[b_heap_size_def] \\
+        rw[ADD_1_SUC, LESS_EQ_IMP_LESS_SUC])
+    >- (imp_res_tac delete_min_size \\
+        rw[b_heap_size_def]));
 
 (* Translations *)
 val _ = translate leaf_def;
